src/Std/Data/DHashMap/Internal/Defs.lean
@@ -171,7 +171,7 @@ namespace Raw₀
 
 /-- Internal implementation detail of the hash map -/
 @[inline] def emptyWithCapacity (capacity := 8) : Raw₀ α β :=
-  ⟨⟨0, mkArray (numBucketsForCapacity capacity).nextPowerOfTwo AssocList.nil⟩,
+  ⟨⟨0, Array.replicate (numBucketsForCapacity capacity).nextPowerOfTwo AssocList.nil⟩,
     by simpa using Nat.pos_of_isPowerOfTwo (Nat.isPowerOfTwo_nextPowerOfTwo _)⟩
 
 @[deprecated emptyWithCapacity (since := "2025-03-12"), inherit_doc emptyWithCapacity]
@@ -191,7 +191,7 @@ def expand [Hashable α] (data : { d : Array (AssocList α β) // 0 < d.size }) 
     { d : Array (AssocList α β) // 0 < d.size } :=
   let ⟨data, hd⟩ := data
   let nbuckets := data.size * 2
-  go 0 data ⟨mkArray nbuckets AssocList.nil, by simpa [nbuckets] using Nat.mul_pos hd Nat.two_pos⟩
+  go 0 data ⟨Array.replicate nbuckets AssocList.nil, by simpa [nbuckets] using Nat.mul_pos hd Nat.two_pos⟩
 where
   /-- Inner loop of `expand`. Copies elements `source[i:]` into `target`,
   destroying `source` in the process. -/
